Arithmetization/Exponential/Pow2.lean
@@ -16,38 +16,38 @@ section IOpen
 
 variable [𝐈open.Mod M]
 
-def IsPow2 (a : M) : Prop := 0 < a ∧ ∀ r ≤ a, 1 < r → r ∣ a → 2 ∣ r
+def Pow2 (a : M) : Prop := 0 < a ∧ ∀ r ≤ a, 1 < r → r ∣ a → 2 ∣ r
 
 def pow2def : Σᴬ[0] 1 :=
   ⟨“0 < #0 ∧ ∀[#0 < #1 + 1] (1 < #0 →  !dvddef [#0, #1] → !dvddef [2, #0])”, by simp [Hierarchy.pi_zero_iff_sigma_zero]⟩
 
-lemma pow2_defined : Σᴬ[0]-Predicate (IsPow2 : M → Prop) pow2def := by
+lemma pow2_defined : Σᴬ[0]-Predicate (Pow2 : M → Prop) pow2def := by
   intro v
   simp [Semiformula.eval_substs, Matrix.comp_vecCons', Matrix.vecHead, Matrix.constant_eq_singleton,
-    IsPow2, pow2def, le_iff_lt_succ, dvd_defined.pval]
+    Pow2, pow2def, le_iff_lt_succ, dvd_defined.pval]
 
-lemma IsPow2.pos {a : M} (h : IsPow2 a) : 0 < a := h.1
+lemma Pow2.pos {a : M} (h : Pow2 a) : 0 < a := h.1
 
-lemma IsPow2.dvd {a : M} (h : IsPow2 a) {r} (hr : r ≤ a) : 1 < r → r ∣ a → 2 ∣ r := h.2 r hr
+lemma Pow2.dvd {a : M} (h : Pow2 a) {r} (hr : r ≤ a) : 1 < r → r ∣ a → 2 ∣ r := h.2 r hr
 
-@[simp] lemma pow2_one : IsPow2 (1 : M) := ⟨by simp, by
+@[simp] lemma pow2_one : Pow2 (1 : M) := ⟨by simp, by
   intro r hr hhr hd
   rcases show r = 0 ∨ r = 1 from le_one_iff_eq_zero_or_one.mp hr with (rfl | rfl)
   · simp
   · simp at hhr⟩
 
-@[simp] lemma not_pow2_zero : ¬IsPow2 (0 : M) := by
+@[simp] lemma not_pow2_zero : ¬Pow2 (0 : M) := by
   intro h; have := h.pos; simp at this
 
-lemma IsPow2.two_dvd {a : M} (h : IsPow2 a) (lt : 1 < a) : 2 ∣ a := h.dvd (le_refl _) lt (by simp)
+lemma Pow2.two_dvd {a : M} (h : Pow2 a) (lt : 1 < a) : 2 ∣ a := h.dvd (le_refl _) lt (by simp)
 
-lemma IsPow2.two_dvd' {a : M} (h : IsPow2 a) (lt : a ≠ 1) : 2 ∣ a :=
+lemma Pow2.two_dvd' {a : M} (h : Pow2 a) (lt : a ≠ 1) : 2 ∣ a :=
   h.dvd (le_refl _) (by
     by_contra A; simp [le_one_iff_eq_zero_or_one] at A
     rcases A with (rfl | rfl) <;> simp at h lt)
     (by simp)
 
-lemma IsPow2.of_dvd {a b : M} (h : b ∣ a) : IsPow2 a → IsPow2 b := by
+lemma Pow2.of_dvd {a b : M} (h : b ∣ a) : Pow2 a → Pow2 b := by
   intro ha
   have : 0 < b := by
     by_contra e
@@ -57,7 +57,7 @@ lemma IsPow2.of_dvd {a b : M} (h : b ∣ a) : IsPow2 a → IsPow2 b := by
   exact ⟨this, fun r hr ltr hb ↦
     ha.dvd (show r ≤ a from le_trans hr (le_of_dvd ha.pos h)) ltr (dvd_trans hb h)⟩
 
-lemma pow2_mul_two {a : M} : IsPow2 (2 * a) ↔ IsPow2 a :=
+lemma pow2_mul_two {a : M} : Pow2 (2 * a) ↔ Pow2 a :=
   ⟨by intro H
       have : ∀ r ≤ a, 1 < r → r ∣ a → 2 ∣ r := by
         intro r hr ltr dvd
@@ -70,10 +70,10 @@ lemma pow2_mul_two {a : M} : IsPow2 (2 * a) ↔ IsPow2 a :=
         · exact hd
         · exact H.dvd (show r ≤ a from le_of_dvd H.pos hd) hr hd⟩⟩
 
-lemma pow2_mul_four {a : M} : IsPow2 (4 * a) ↔ IsPow2 a := by
+lemma pow2_mul_four {a : M} : Pow2 (4 * a) ↔ Pow2 a := by
   simp [←two_mul_two_eq_four, mul_assoc, pow2_mul_two]
 
-lemma IsPow2.elim {p : M} : IsPow2 p ↔ p = 1 ∨ ∃ q, p = 2 * q ∧ IsPow2 q :=
+lemma Pow2.elim {p : M} : Pow2 p ↔ p = 1 ∨ ∃ q, p = 2 * q ∧ Pow2 q :=
   ⟨by intro H
       by_cases hp : 1 < p
       · have : 2 ∣ p := H.two_dvd hp
@@ -83,24 +83,24 @@ lemma IsPow2.elim {p : M} : IsPow2 p ↔ p = 1 ∨ ∃ q, p = 2 * q ∧ IsPow2 q
         left; exact this,
    by rintro (rfl | ⟨q, rfl, hq⟩) <;> simp [pow2_one, pow2_mul_two, *]⟩
 
-@[simp] lemma pow2_two : IsPow2 (2 : M) := IsPow2.elim.mpr (Or.inr ⟨1, by simp⟩)
+@[simp] lemma pow2_two : Pow2 (2 : M) := Pow2.elim.mpr (Or.inr ⟨1, by simp⟩)
 
-lemma IsPow2.div_two {p : M} (h : IsPow2 p) (ne : p ≠ 1) : IsPow2 (p /ₑ 2) := by
-  rcases IsPow2.elim.mp h with (rfl | ⟨q, rfl, pq⟩)
+lemma Pow2.div_two {p : M} (h : Pow2 p) (ne : p ≠ 1) : Pow2 (p /ₑ 2) := by
+  rcases Pow2.elim.mp h with (rfl | ⟨q, rfl, pq⟩)
   · simp at ne
   simpa
 
-lemma IsPow2.two_mul_div_two {p : M} (h : IsPow2 p) (ne : p ≠ 1) : 2 * (p /ₑ 2) = p := by
-  rcases IsPow2.elim.mp h with (rfl | ⟨q, rfl, _⟩)
+lemma Pow2.two_mul_div_two {p : M} (h : Pow2 p) (ne : p ≠ 1) : 2 * (p /ₑ 2) = p := by
+  rcases Pow2.elim.mp h with (rfl | ⟨q, rfl, _⟩)
   · simp at ne
   simp
 
-lemma IsPow2.div_two_mul_two {p : M} (h : IsPow2 p) (ne : p ≠ 1) : (p /ₑ 2) * 2 = p := by
+lemma Pow2.div_two_mul_two {p : M} (h : Pow2 p) (ne : p ≠ 1) : (p /ₑ 2) * 2 = p := by
   simp [mul_comm, h.two_mul_div_two ne]
 
-lemma IsPow2.elim' {p : M} : IsPow2 p ↔ p = 1 ∨ 1 < p ∧ ∃ q, p = 2 * q ∧ IsPow2 q := by
+lemma Pow2.elim' {p : M} : Pow2 p ↔ p = 1 ∨ 1 < p ∧ ∃ q, p = 2 * q ∧ Pow2 q := by
   by_cases hp : 1 < p <;> simp [hp]
-  · exact IsPow2.elim
+  · exact Pow2.elim
   · have : p = 0 ∨ p = 1 := le_one_iff_eq_zero_or_one.mp (show p ≤ 1 from by simpa using hp)
     rcases this with (rfl | rfl) <;> simp
 
@@ -175,64 +175,64 @@ section ISigma₀
 
 variable [𝐈𝚺₀.Mod M]
 
-namespace IsPow2
+namespace Pow2
 
-lemma mul {a b : M} (ha : IsPow2 a) (hb : IsPow2 b) : IsPow2 (a * b) := by
+lemma mul {a b : M} (ha : Pow2 a) (hb : Pow2 b) : Pow2 (a * b) := by
   wlog hab : a ≤ b
   · simpa [mul_comm] using this hb ha (by simp at hab; exact LT.lt.le hab)
   refine hierarchy_order_induction₀ M Σ 0
-    (fun b ↦ ∀ a ≤ b, IsPow2 a → IsPow2 b → IsPow2 (a * b))
+    (fun b ↦ ∀ a ≤ b, Pow2 a → Pow2 b → Pow2 (a * b))
     ⟨⟨“∀[#0 < #1 + 1] (!pow2def [#0] → !pow2def [#1] → !pow2def [#0 * #1])”, by simp⟩,
      by intro v; simp [le_iff_lt_succ, Semiformula.eval_substs, Matrix.vecHead, pow2_defined.pval]⟩ ?_ b a hab ha hb
   simp; intro b H a hab ha hb
-  have : a = 1 ∨ 1 < a ∧ ∃ a', a = 2 * a' ∧ IsPow2 a' := IsPow2.elim'.mp ha
+  have : a = 1 ∨ 1 < a ∧ ∃ a', a = 2 * a' ∧ Pow2 a' := Pow2.elim'.mp ha
   rcases this with (rfl | ⟨lta, a, rfl, ha⟩)
   · simpa using hb
-  · have : b = 1 ∨ 1 < b ∧ ∃ b', b = 2 * b' ∧ IsPow2 b' := IsPow2.elim'.mp hb
+  · have : b = 1 ∨ 1 < b ∧ ∃ b', b = 2 * b' ∧ Pow2 b' := Pow2.elim'.mp hb
     rcases this with (rfl | ⟨ltb, b, rfl, hb⟩)
     · simpa using ha
     · have ltb : b < 2 * b := lt_two_mul_self (pos_iff_ne_zero.mpr $ by rintro rfl; simp at ltb)
       have hab : a ≤ b := le_of_mul_le_mul_left hab (by simp)
-      have : IsPow2 (a * b) := H b ltb a hab (by assumption) (by assumption)
-      suffices : IsPow2 (4 * a * b)
+      have : Pow2 (a * b) := H b ltb a hab (by assumption) (by assumption)
+      suffices : Pow2 (4 * a * b)
       · have : (2 * a) * (2 * b) = 4 * a * b := by simp [mul_assoc, mul_left_comm a 2 b, ←two_mul_two_eq_four]
         simpa [this]
       simpa [mul_assoc, pow2_mul_four] using this
 
-@[simp] lemma mul_iff {a b : M} : IsPow2 (a * b) ↔ IsPow2 a ∧ IsPow2 b :=
+@[simp] lemma mul_iff {a b : M} : Pow2 (a * b) ↔ Pow2 a ∧ Pow2 b :=
   ⟨fun h ↦ ⟨h.of_dvd (by simp), h.of_dvd (by simp)⟩, by rintro ⟨ha, hb⟩; exact ha.mul hb⟩
 
-@[simp] lemma sq_iff {a : M} : IsPow2 (a^2) ↔ IsPow2 a := by
+@[simp] lemma sq_iff {a : M} : Pow2 (a^2) ↔ Pow2 a := by
   simp [_root_.sq]
 
-lemma sq {a : M} : IsPow2 a → IsPow2 (a^2) := by
+lemma sq {a : M} : Pow2 a → Pow2 (a^2) := by
   simp [_root_.sq]
 
-lemma dvd_of_le {a b : M} (ha : IsPow2 a) (hb : IsPow2 b) : a ≤ b → a ∣ b := by
+lemma dvd_of_le {a b : M} (ha : Pow2 a) (hb : Pow2 b) : a ≤ b → a ∣ b := by
   intro hab
-  refine hierarchy_order_induction₀ M Σ 0 (fun b ↦ ∀ a ≤ b, IsPow2 a → IsPow2 b → a ∣ b)
+  refine hierarchy_order_induction₀ M Σ 0 (fun b ↦ ∀ a ≤ b, Pow2 a → Pow2 b → a ∣ b)
     ⟨⟨“∀[#0 < #1 + 1] (!pow2def [#0] → !pow2def [#1] → !dvddef [#0, #1]) ”, by simp⟩,
       by intro v; simp [le_iff_lt_succ, Semiformula.eval_substs, Matrix.vecHead, pow2_defined.pval, dvd_defined.pval]⟩
     ?_ b a hab ha hb
   simp; intro b H a hab ha hb
-  have : b = 1 ∨ 1 < b ∧ ∃ b', b = 2 * b' ∧ IsPow2 b' := IsPow2.elim'.mp hb
+  have : b = 1 ∨ 1 < b ∧ ∃ b', b = 2 * b' ∧ Pow2 b' := Pow2.elim'.mp hb
   rcases this with (rfl | ⟨ltb, b, rfl, hb⟩)
   · rcases le_one_iff_eq_zero_or_one.mp hab with (rfl | rfl) <;> simp
     · simp at ha
-  · have : a = 1 ∨ 1 < a ∧ ∃ a', a = 2 * a' ∧ IsPow2 a' := IsPow2.elim'.mp ha
+  · have : a = 1 ∨ 1 < a ∧ ∃ a', a = 2 * a' ∧ Pow2 a' := Pow2.elim'.mp ha
     rcases this with (rfl | ⟨lta, a, rfl, ha⟩)
     · simp
     · have ltb : b < 2 * b := lt_two_mul_self (pos_iff_ne_zero.mpr $ by rintro rfl; simp at ltb)
       have hab : a ≤ b := le_of_mul_le_mul_left hab (by simp)
       exact mul_dvd_mul_left 2 <| H b ltb a hab (by assumption) (by assumption)
 
-lemma le_iff_dvd {a b : M} (ha : IsPow2 a) (hb : IsPow2 b) : a ≤ b ↔ a ∣ b :=
-  ⟨IsPow2.dvd_of_le ha hb, le_of_dvd hb.pos⟩
+lemma le_iff_dvd {a b : M} (ha : Pow2 a) (hb : Pow2 b) : a ≤ b ↔ a ∣ b :=
+  ⟨Pow2.dvd_of_le ha hb, le_of_dvd hb.pos⟩
 
-lemma two_le {a : M} (pa : IsPow2 a) (ne1 : a ≠ 1) : 2 ≤ a :=
+lemma two_le {a : M} (pa : Pow2 a) (ne1 : a ≠ 1) : 2 ≤ a :=
   le_of_dvd pa.pos (pa.two_dvd' ne1)
 
-lemma le_iff_lt_two {a b : M} (ha : IsPow2 a) (hb : IsPow2 b) : a ≤ b ↔ a < 2 * b := by
+lemma le_iff_lt_two {a b : M} (ha : Pow2 a) (hb : Pow2 b) : a ≤ b ↔ a < 2 * b := by
   constructor
   · intro h; exact lt_of_le_of_lt h (lt_two_mul_self hb.pos)
   · intro h
@@ -246,26 +246,26 @@ lemma le_iff_lt_two {a b : M} (ha : IsPow2 a) (hb : IsPow2 b) : a ≤ b ↔ a < 
           simpa [ha.two_mul_div_two ea] using dvd_of_le ha (by simpa using hb) (LT.lt.le h)
         exact (mul_dvd_mul_iff_left (by simp)).mp this
       rcases this with ⟨b', rfl⟩
-      have hb' : IsPow2 b' := by simp at hb; exact hb.2
+      have hb' : Pow2 b' := by simp at hb; exact hb.2
       have : 2 ∣ b' := hb'.two_dvd' (by rintro rfl; simp [ha.two_mul_div_two ea] at h)
       rcases this with ⟨b'', rfl⟩
       simp [←mul_assoc, ha.div_two_mul_two ea]
 
-lemma lt_iff_two_mul_le {a b : M} (ha : IsPow2 a) (hb : IsPow2 b) : a < b ↔ 2 * a ≤ b := by
+lemma lt_iff_two_mul_le {a b : M} (ha : Pow2 a) (hb : Pow2 b) : a < b ↔ 2 * a ≤ b := by
   by_cases eb : b = 1
   · simp [eb, ←lt_two_iff_le_one]
   · rw [←hb.two_mul_div_two eb]; simp [le_iff_lt_two ha (hb.div_two eb)]
 
-lemma sq_or_dsq {a : M} (pa : IsPow2 a) : ∃ b, a = b^2 ∨ a = 2 * b^2 := by
+lemma sq_or_dsq {a : M} (pa : Pow2 a) : ∃ b, a = b^2 ∨ a = 2 * b^2 := by
   suffices : ∃ b ≤ a, a = b^2 ∨ a = 2 * b^2
   · rcases this with ⟨b, _, h⟩
     exact ⟨b, h⟩
-  refine hierarchy_order_induction₀ M Σ 0 (fun a ↦ IsPow2 a → ∃ b ≤ a, a = b^2 ∨ a = 2 * b^2)
+  refine hierarchy_order_induction₀ M Σ 0 (fun a ↦ Pow2 a → ∃ b ≤ a, a = b^2 ∨ a = 2 * b^2)
     ⟨⟨“!pow2def [#0] → ∃[#0 < #1 + 1] (#1 = #0 * #0 ∨ #1 = 2 * (#0 * #0)) ”, by simp⟩,
       by intro v; simp [←le_iff_lt_succ, Semiformula.eval_substs, pow2_defined.pval, Matrix.vecHead, _root_.sq]⟩
     ?_ a pa
   simp; intro a IH pa
-  rcases IsPow2.elim'.mp pa with (rfl | ⟨ha, a, rfl, pa'⟩)
+  rcases Pow2.elim'.mp pa with (rfl | ⟨ha, a, rfl, pa'⟩)
   · exact ⟨1, by simp⟩
   · have : 0 < a := by simpa [←pos_iff_one_le] using one_lt_iff_two_le.mp ha
     rcases IH a (lt_mul_of_one_lt_left this one_lt_two) pa' with ⟨b, _, (rfl | rfl)⟩
@@ -273,28 +273,28 @@ lemma sq_or_dsq {a : M} (pa : IsPow2 a) : ∃ b, a = b^2 ∨ a = 2 * b^2 := by
     · exact ⟨2 * b, by simp; exact le_trans (by simp) le_two_mul_left,
       by left; simp [_root_.sq, mul_assoc, mul_left_comm]⟩
 
-lemma sqrt {a : M} (h : IsPow2 a) (hsq : (√a)^2 = a) : IsPow2 (√a) := by
+lemma sqrt {a : M} (h : Pow2 a) (hsq : (√a)^2 = a) : Pow2 (√a) := by
   rw [←hsq] at h; simpa using h
 
-@[simp] lemma IsPow2.not_three : ¬IsPow2 (3 : M) := by
+@[simp] lemma Pow2.not_three : ¬Pow2 (3 : M) := by
   intro h
   have : 2 ∣ 3 := h.two_dvd (by simp [←two_add_one_eq_three])
   simp [←two_add_one_eq_three, ←remainder_eq_zero_iff_dvd, one_lt_two] at this
 
-lemma four_le {i : M} (hi : IsPow2 i) (lt : 2 < i) : 4 ≤ i := by
+lemma four_le {i : M} (hi : Pow2 i) (lt : 2 < i) : 4 ≤ i := by
   by_contra A
   have : i ≤ 3 := by simpa [←three_add_one_eq_four, ←le_iff_lt_succ] using A
   rcases le_three_iff_eq_zero_or_one_or_two_or_three.mp this with (rfl | rfl | rfl | rfl) <;> simp at lt hi
 
-end IsPow2
+end Pow2
 
-lemma LenBit.remainder_pow2 {a i j : M} (pi : IsPow2 i) (pj : IsPow2 j) (h : i < j) : LenBit i (a mod j) ↔ LenBit i a :=
-  LenBit.remainder (by rw [←IsPow2.le_iff_dvd] <;> simp [pi, pj, ←IsPow2.lt_iff_two_mul_le, h])
+lemma LenBit.remainder_pow2 {a i j : M} (pi : Pow2 i) (pj : Pow2 j) (h : i < j) : LenBit i (a mod j) ↔ LenBit i a :=
+  LenBit.remainder (by rw [←Pow2.le_iff_dvd] <;> simp [pi, pj, ←Pow2.lt_iff_two_mul_le, h])
 
-lemma LenBit.add_pow2 {a i j : M} (pi : IsPow2 i) (pj : IsPow2 j) (h : i < j) : LenBit i (a + j) ↔ LenBit i a :=
-  LenBit.add (by rw [←IsPow2.le_iff_dvd] <;> simp [pi, pj, ←IsPow2.lt_iff_two_mul_le, h])
+lemma LenBit.add_pow2 {a i j : M} (pi : Pow2 i) (pj : Pow2 j) (h : i < j) : LenBit i (a + j) ↔ LenBit i a :=
+  LenBit.add (by rw [←Pow2.le_iff_dvd] <;> simp [pi, pj, ←Pow2.lt_iff_two_mul_le, h])
 
-lemma LenBit.add_pow2_iff {a i j : M} (pi : IsPow2 i) (pj : IsPow2 j) (h : a < j) : LenBit i (a + j) ↔ i = j ∨ LenBit i a := by
+lemma LenBit.add_pow2_iff {a i j : M} (pi : Pow2 i) (pj : Pow2 j) (h : a < j) : LenBit i (a + j) ↔ i = j ∨ LenBit i a := by
   rcases show i < j ∨ i = j ∨ i > j from lt_trichotomy i j with (hij | rfl | hij)
   · simp [LenBit.add_pow2 pi pj hij, hij.ne]
   · simp [LenBit.add_self h]
